src/tactic/nccc/lit.lean
@@ -14,19 +14,36 @@ def neg : lit → lit
 | ⟨b, k, ts⟩ := ⟨bnot b, k, ts⟩
 
 def holds (M : model α) (v : nat → α) : lit → Prop
-| ⟨tt, k, ts⟩  :=    M.rels k (ts.map (term.val M v))
-| ⟨ff, k, ts⟩  :=  ¬ M.rels k (ts.map (term.val M v))
+| ⟨tt, k, ts⟩  :=    M.rels k (ts.map (term.value M v))
+| ⟨ff, k, ts⟩  :=  ¬ M.rels k (ts.map (term.value M v))
 
-def repr : lit → string
-| ⟨s, k, ts⟩ :=
-  (if s then "" else "¬") ++ "P" ++ k.to_subs ++
-  (list.foldl (λ s1 s2, s1 ++ " " ++ s2) "" (ts.map term.repr))
+lemma holds_neg (M : model α) (v : nat → α) (l : lit) :
+  holds M v l.neg ↔ ¬ holds M v l :=
+by { cases l with b; cases b; 
+     simp only [bnot, neg, holds, list.map, classical.not_not] }
 
-instance has_repr : has_repr lit := ⟨repr⟩
-
-meta instance has_to_format : has_to_format lit := ⟨λ x, repr x⟩
+-- def repr : lit → string
+-- | ⟨s, k, ts⟩ :=
+--   (if s then "" else "¬") ++ "P" ++ k.to_subs ++
+--   (list.foldl (λ s1 s2, s1 ++ " " ++ s2) "" (ts.map term.repr))
+-- 
+-- instance has_repr : has_repr lit := ⟨repr⟩
+-- 
+-- meta instance has_to_format : has_to_format lit := ⟨λ x, repr x⟩
 
 def vdxs : lit → list nat 
 | ⟨_, _, ts⟩ := ⋃ (ts.map term.vdxs)
+
+def subst (σ : sub) : lit → lit
+| ⟨b, m, ts⟩ := ⟨b, m, ts.map (term.subst σ)⟩ 
+
+lemma holds_subst (M : model α) (v : nat → α) (σ : sub) (l : lit) :
+  holds M v (l.subst σ) ↔ holds M (val.subst M v σ) l :=  
+begin
+  cases l with b k ts, cases b;
+  simp only [holds, subst, val.subst, 
+    list.map_map, term.value_comp_subst],
+end
+
 
 end lit
