src/tactic/nccc/mat.lean
@@ -1,5 +1,7 @@
 import .form
 
+variable {α : Type}
+
 local notation  `⊤*` := form.true
 local notation  `⊥*` := form.false
 local notation  `⟪` l `⟫` := form.lit l
@@ -8,14 +10,43 @@ local notation  p `∧*` q := form.and p q
 local notation  `∀*` := form.fa
 local notation  `∃*` := form.ex
 
-@[reducible] def mat : Type := list (list lit)
+@[reducible] def cla : Type := list lit
+
+namespace cla
+
+def is_pos (C : cla) : bool := C.all lit.sign
+
+def vdxs (C : cla) : list nat := ⋃ (C.map lit.vdxs)
+
+def holds (M : model α) (v : nat → α) (c : cla) : Prop :=
+∀ l ∈ c, lit.holds M v l
+
+def subst : sub → cla → cla :=
+list.map ∘ lit.subst 
+
+lemma holds_subst {M : model α} {v : nat → α} {σ : sub} {c : cla} :
+  holds M v (c.subst σ) ↔ holds M (val.subst M v σ) c :=  
+begin
+  constructor; intros h1 l h2,
+  { rw ← lit.holds_subst, apply h1, 
+    apply list.mem_map_of_mem _ h2 },
+  { have h3 : ∃ x, x ∈ c ∧ lit.subst σ x = l,
+    { rw ← list.mem_map, exact h2 },
+    rcases h3 with ⟨x, h3, h4⟩, 
+    rw [←h4, lit.holds_subst],
+    apply h1 _ h3 } 
+end
+  
+end cla
+
+
+
+@[reducible] def mat : Type := list cla
 
 namespace mat
 
-variable {α : Type}
-
-def holds (M : model α) (v : nat → α) (m : mat) : Prop :=
-∃ c ∈ m, ∀ l ∈ c, lit.holds M v l
+def holds (M : model α) (v : nat → α) (A : mat) : Prop :=
+∃ C ∈ A, cla.holds M v C
 
 def valsat (α m) : Prop :=
 ∀ M : model α, ∃ v : nat → α, (holds M v m)
@@ -33,3 +64,9 @@ def dnf : form → mat
 
 lemma form_valsat_of_mat_valsat (α : Type) (p : form) :
   p.quant_free → (dnf p).valsat α → p.valsat α := sorry
+
+
+
+
+
+
