src/tactic/nccc/model.lean
@@ -2,16 +2,11 @@ variables {α β : Type}
 
 structure model (α : Type) :=
 (inhab : α)
-(funcs : nat → list α → α)
+(funs  : nat → list α → α)
 (rels  : nat → list α → Prop)
-
---def func.default [inhabited α] (as : list α) : α :=
---@inhabited.default _ _
---
---def rel.default (as : list α) : Prop := false
 
 def model.default (α : Type) [inhabited α] : model α :=
 let a := inhabited.default α in
 { inhab := a,
-  funcs := λ _ _, a,
+  funs  := λ _ _, a,
   rels  := λ _ _, false }
