src/tactic/nccc/proof.lean
@@ -1,67 +1,288 @@
-import .mat
+import .search .logic tactic.mono_con
 
-@[reducible] def cla : Type := list lit
+variable {α : Type}
 
-@[reducible] def sub : Type := list (nat × term)
+local notation `⅋` k   := term.fnc k
+local notation t `&` s := term.tpp t s
+local notation t `#` k := term.vpp t k
 
-local notation  `#` := term.var
-local notation  `&` := term.fnc
-local notation  t1 `^*` t2 := term.app t1 t2
+def goal : Type := cla × cla × mat
+def ext_goal : Type := cla × cla × mat × mat
 
-def cla.is_pos (C : cla) : bool := C.all lit.sign
+namespace goal
 
-def cla.vdxs (C : cla) : list nat := ⋃ (C.map lit.vdxs)
+def is_ext (m x : mat) : Prop :=
+∀ c ∈ x, ∃ d ∈ m, ∃ σ : sub, c = cla.subst σ d
 
-def sub.term_app_aux (k : nat) : sub → term
-| []         := #k
-| ((m,t)::σ) :=
-  if k = m then t else sub.term_app_aux σ
+lemma is_ext_of_subset_of_is_ext {m n x : mat} : 
+  m ⊆ n → is_ext m x → is_ext n x :=
+begin
+  intros h1 h2 c h3,
+  rcases (h2 _ h3) with ⟨d, h4, σ, h5⟩, 
+  refine ⟨d, h1 h4, σ, h5⟩,
+end
 
-def sub.term_app (σ : sub) : term → term
-| (# k) := sub.term_app_aux k σ
-| (& k) := & k
-| (t ^* s) := (sub.term_app t) ^* (sub.term_app s)
+def ext_holds (M : model α) (v : nat → α) : ext_goal → Prop 
+| (p, c, m, x) := 
+  (∃ l ∈ p, lit.holds M v l) ∨ 
+  (∀ l ∈ c, lit.holds M v l) ∨ 
+  (∃ d ∈ m, cla.holds M v d) ∨ 
+  (∃ d ∈ x, cla.holds M v d) 
 
-def sub.lit_app (σ : sub) : lit → lit
-| ⟨b, m, ts⟩ := ⟨b, m, ts.map σ.term_app⟩
+def ext_valid (α : Type) : goal → Prop 
+| (p, c, m) := 
+  ∃ x : mat, is_ext m x ∧ 
+    (∀ M : model α, ∀ v : nat → α, ext_holds M v (p, c, m, x))
 
-inductive proof : cla → mat → cla → Type
-| axm {M : mat} {P : cla} : proof [] M P
+open list
+
+lemma mat.exv_of_holds_ext {M : model α} {v : nat → α} {m x : mat} :
+  is_ext m x → x.holds M v → (∃ w : nat → α, m.holds M w) := 
+begin
+  intros h1 h2, 
+  rcases h2 with ⟨c, h2, h3⟩,  
+  rcases (h1 _ h2) with ⟨d, h4, σ, h5⟩,
+  refine ⟨val.subst M v σ, d, h4, _⟩, 
+  rw [←cla.holds_subst, ←h5], exact h3
+end
+
+lemma start_none_correct (m : mat) (j : nat) (h1 : j < m.length) :
+  ext_valid α ([], m.nth_le j h1, m.except j) → m.valsat α := 
+begin
+  intros h2 M, 
+  rcases h2 with ⟨x, h2, h3⟩, 
+  cases h3 M (λ _, M.inhab) with h4 h4, 
+  { rcases h4 with ⟨_, h4, _⟩, cases h4 },
+  cases h4, 
+  refine ⟨(λ _, M.inhab), _, nth_le_mem _ _ _, h4⟩,
+  cases h4,
+  { rcases h4 with ⟨d, h5, h6⟩, 
+    refine ⟨(λ _, M.inhab), _, except_subset_self h5, h6⟩ },
+  apply mat.exv_of_holds_ext 
+    (is_ext_of_subset_of_is_ext except_subset_self h2) h4,
+end
+
+lemma start_some_correct (m : mat) (j : nat) (h1 : j < m.length) (σ : sub) :
+  ext_valid α ([], (m.nth_le j h1).subst σ, m) → m.valsat α := 
+begin
+  intros h2 M, 
+  rcases h2 with ⟨x, h2, h3⟩, 
+  cases h3 M (λ _, M.inhab) with h4 h4, 
+  { rcases h4 with ⟨_, h4, _⟩, cases h4 },
+  cases h4,
+  { refine ⟨val.subst M (λ _, M.inhab) σ, 
+    m.nth_le j h1, nth_le_mem _ _ _, _⟩, 
+    rw [←cla.holds_subst], exact h4 },
+  cases h4, 
+  { rcases h4 with ⟨d, h5, h6⟩, 
+    refine ⟨(λ _, M.inhab), _, h5, h6⟩ },
+  apply mat.exv_of_holds_ext h2 h4,
+end
+
+lemma red_correct (l : lit) (c : cla) (m : mat) (p : cla) :
+  l.neg ∈ p → ext_valid α (p, c, m) → ext_valid α (p, l :: c, m) := 
+begin
+  intro h1, 
+  mono_con with x ⟨ | M v ⟩,  
+  exact id, simp only,
+  intro h2, cases h2, 
+  { left, exact h2 },
+  { cases h2 with h2 h3,
+    { cases classical.em (l.holds M v) with h4 h4,
+      { right, left, rw forall_mem_cons,
+        constructor; assumption },
+      { left, refine ⟨l.neg, h1, _⟩, 
+        rw lit.holds_neg, exact h4 } },
+    right, right, exact h3 }
+end
+
+#exit
+def holds (M : model α) (v : nat → α) : goal → Prop 
+| (c, m, p) := (cla.holds M v c ∨ ∃ d ∈ m, cla.holds M v d) ∧ (∀ l ∈ p, ¬ lit.holds M v l)
+
+def valsat (α : Type) (g : goal) : Prop :=
+∀ M : model α, ∃ v : nat → α, (holds M v g)
+
+end goal
+
+open list
+
+#check tactic.interactive.rcades
+lemma start_none_correct (m : mat) (j : nat) (h1 : j < m.length) :
+  goal.valsat α (m.nth_le j h1, m.except j, []) → m.valsat α := 
+begin
+  intros h2 M, 
+  rcases (h2 M) with ⟨v, h3, h4⟩, 
+  refine ⟨v, _⟩, cases h3,
+  { refine ⟨_, nth_le_mem _ _ _, h3⟩ },
+  { rcases h3 with ⟨c, h5, h6⟩,
+    refine ⟨c, mem_of_mem_except h5, h6⟩ }
+end
+
+lemma start_some_correct (m : mat) (j : nat) (h1 : j < m.length) (σ : sub) :
+  goal.valsat α ((m.nth_le j h1).subst σ, m, []) → m.valsat α := 
+begin
+  intros h2 M, 
+  rcases (h2 M) with ⟨v, h3, h4⟩, 
+  cases h3,
+  refine ⟨val.subst M v σ, m.nth_le j h1, 
+    nth_le_mem _ _ _, cla.holds_subst.elim_left h3⟩,
+  refine ⟨v, h3⟩,
+end
+
+lemma red_correct (l : lit) (c : cla) (m : mat) (p : cla) :
+  l.neg ∈ p → goal.valsat α (c, m, p) → goal.valsat α (l :: c, m, p) := 
+begin
+  intros h1 h2 M,
+  rcases h2 M with ⟨v, h3, h4⟩,
+  refine ⟨v, _, h4⟩,
+  cases h3 with h5 h6,
+  { left, 
+    apply list.forall_mem_cons.elim_right ⟨ _, h5⟩,
+    apply classical.not_not.elim_left,
+    rw ← lit.holds_neg,
+    exact h4 _ h1 },
+  { right, exact h6 }
+end
+
+lemma ext_none_correct (l : lit) (c : cla) (m : mat) (p : cla) 
+  (i j : nat) (h1 : j < m.length) (h2 : i < (m.nth_le j h1).length) : 
+  l.neg = (m.nth_le j h1).nth_le i h2 → 
+  goal.valsat α (c, m, p) → 
+  goal.valsat α ((m.nth_le j h1).except i, m.except j, l :: p) → 
+  goal.valsat α (l :: c, m, p) :=  sorry
+
+
+
+#exit
+
+
+inductive rule : Type
+| start : nat → option sub → rule 
+| red   : rule
+| ext   : nat → nat → option sub → rule 
+
+def goal : Type := option cla × mat × cla
+
+open rule 
+
+def check : list rule → list goal → bool 
+| (r :: rs) ((some [], _, _) :: gs) := check rs gs
+| (start j none :: rs) [(none, M, [])] :=  
+  if h : j < M.length
+  then check rs [((M.nth_le j h), (M.except j), [])] 
+  else ff
+| (start j (some σ) :: rs) [(none, M, [])] :=  
+  if h : j < M.length
+  then check rs [((M.nth_le j h).subst σ, M, [])] 
+  else ff
+| (red :: rs) ((some (L :: C), M, P) :: gs) := 
+  if L.neg ∈ P
+  then check rs ((some C, M, P) :: gs) 
+  else ff
+| (ext j i none :: rs) ((some (L :: C), M, P) :: gs) :=  
+  if h1 : j < M.length 
+  then if h2 : i < (M.nth_le j h1).length
+       then let D := M.nth_le j h1 in 
+            let N := D.nth_le i h2 in
+            (N = L.neg) && 
+              check rs ((C, M, P) :: (D.except i, M.except j, L :: P) :: gs)
+       else ff
+  else ff
+| (ext j i (some σ) :: rs) ((some (L :: C), M, P) :: gs) :=  
+  if h1 : j < M.length 
+  then if h2 : i < (M.nth_le j h1).length
+       then let D := M.nth_le j h1 in 
+            let Dσ := D.subst σ in
+            let Nσ := (D.nth_le i h2).subst σ  in
+            (Nσ = L.neg) && 
+              check rs ((C, M, P) :: (D.except i, M, L :: P) :: gs)
+       else ff
+  else ff
+
+#print axioms check
+
+
+#exit
+
+
+| (rule.start j (some σx) :: rs) none M [] := 
+  do ⟨_, h⟩ ← get_lt_proof j M.length,
+     σ ← σx.inst,
+     (rs', π) ← of_rules rs ((M.nth_le j h).subst σ) M [],
+     return (rs', proof.start' π)
+
+
+#exit
+inductive proof : option cla → mat → cla → Type
+| start {M : mat} {j : nat} {h : j < M.length} :
+  proof (M.nth_le j h) (M.except j) [] → 
+  proof none M []
+| start' {M : mat} {j : nat} {h : j < M.length} {σ : sub} :
+  proof ((M.nth_le j h).subst σ) M [] → 
+  proof none M []
 | red {M : mat} {C P : cla} {L : lit} :
   L.neg ∈ P → proof C M P → proof (L::C) M P
-| ext {M : mat} {C P : cla} {L : lit} (C₁ : cla) :
-  C₁ ∈ M → proof C M P →
-  proof (C₁.erase L.neg) (M.erase C₁) (L::P) →
+| ext {M : mat} {C P : cla} {L : lit} (i j : nat) 
+  {h1 : j < M.length} {h2 : i < (M.nth_le j h1).length} :
+  let D := M.nth_le j h1 in
+  let N := D.nth_le i h2 in
+  proof C M P → 
+  N = L.neg → 
+  proof (D.except i) (M.except j) (L::P) →
   proof (L::C) M P
-| cxt {M : mat} {C P : cla} (C₁ : cla) (L : lit) (σ : sub) :
-  C₁ ∈ M → proof C M P →
-  proof ((C₁.map (σ.lit_app)).erase L.neg) M (L::P) →
+| ext' {M : mat} {C P : cla} {L : lit} {σ : sub} {i j : nat}
+  {h1 : j < M.length} {h2 : i < (M.nth_le j h1).length} :
+  let D := (M.nth_le j h1).subst σ in
+  let N := ((M.nth_le j h1).nth_le i h2).subst σ in
+  proof C M P → 
+  N = L.neg → 
+  proof (D.except i) M (L::P) →
   proof (L::C) M P
+| axm {M : mat} {P : cla} : proof (some []) M P
 
+open tactic
+
+meta def get_lt_proof (m n : nat) : tactic (@subtype unit (λ _, m < n)) := 
+if h : m < n then return (subtype.mk () h) else failed
+
+meta def get_proof (P : Prop) [decidable P] : tactic (@subtype unit (λ _, P)) := 
+if h : P then return (subtype.mk () h) else failed
+
+meta def subx.inst_aux (ktx : nat × expr) : tactic (nat × term) :=
+do t ← eval_expr term ktx.snd, return (ktx.fst, t)
+
+meta def subx.inst (σx : subx) : tactic sub :=
+monad.mapm subx.inst_aux σx 
+
+meta def of_rules : list rule → ∀ C : option cla, 
+  ∀ M : mat, ∀ P : cla, tactic (list rule × proof C M P)
+| (rule.start j none :: rs) none M [] := 
+  do ⟨_, h⟩ ← get_lt_proof j M.length,
+     (rs', π) ← of_rules rs (M.nth_le j h) (M.except j) [],
+     return (rs', proof.start π) 
+| (rule.start j (some σx) :: rs) none M [] := 
+  do ⟨_, h⟩ ← get_lt_proof j M.length,
+     σ ← σx.inst,
+     (rs', π) ← of_rules rs ((M.nth_le j h).subst σ) M [],
+     return (rs', proof.start' π)
+| (rule.red :: rs) (some (L::C)) M P := 
+  do ⟨_, h⟩ ← get_proof (L.neg ∈ P),
+     (rs', π) ← of_rules rs (some C) M P,
+     return (rs', proof.red h π)
 
 
 
 #exit
-open expr tactic
-
-meta def foo : tactic unit :=
-do m ← tactic.mk_meta_var `(term),
-  trace m,
-  (unify m `(term.var 0) >> trace m >> failed) <|>
-  (trace m >> skip)
-
-example : false := by foo
-
-
+  if h : j < M.length
+  then do (rs', π) ← of_rules rs (M.nth_le j h) (M.except j) [],
+          return (rs', proof.start π) 
+  else failed
 
 #exit
+--lemma valsat_goal_of_proof {α : Type} (M : mat)  :
+--  proof none M [] → M.valsat α := sorry
 
-def sub.term_app : sub → term → term
-| (# _)    := 0
-| (& n)    := n + 1
-| (t ^* s) := max (fresh_sdx t) (fresh_sdx s)
-
-
-def sub.lit_app (σ : sub) (l : lit) : lit :=
-
-#exit
+lemma valsat_of_proof {α : Type} (M : mat) :
+  proof none M [] → M.valsat α := sorry
+  
