src/tactic/nccc/term.lean
@@ -6,85 +6,166 @@ open tactic
 
 @[derive has_reflect, derive decidable_eq]
 inductive term : Type
-| var : nat → term
 | fnc : nat → term
-| app : term → term → term
+| tpp : term → term → term
+| vpp : term → nat → term
 
-local notation  `#` := term.var
-local notation  `&` := term.fnc
-local notation  t `^*` s := term.app t s
+local notation `⅋` k   := term.fnc k
+local notation t `&` s := term.tpp t s
+local notation t `#` k := term.vpp t k
 
 namespace term
 
-def repr : term → string
-| (# k) := "X" ++ k.to_subs
-| (& k) := "C" ++ k.to_subs
-| (t ^* s) := "(" ++ t.repr ++ " " ++ s.repr ++ ")"
+-- def repr : term → string
+-- | (# k) := "X" ++ k.to_subs
+-- | (& k) := "C" ++ k.to_subs
+-- | (t ^* s) := "(" ++ t.repr ++ " " ++ s.repr ++ ")"
+-- 
+-- instance has_repr : has_repr term := ⟨repr⟩
+-- 
+-- meta instance has_to_format : has_to_format term := ⟨λ x, repr x⟩
+-- 
+-- def mk_app (t : term) (ts : list term) : term :=
+-- list.foldl app t ts
+-- 
+-- def symb_arity_core (k : nat) : nat → term → option (bool × nat)
+-- | m (# _)    := none
+-- | m (& n)    := if k = n then some (ff,m) else none
+-- | m (t ^* s) :=
+--   symb_arity_core (m+1) t <|> symb_arity_core 0 s
 
-instance has_repr : has_repr term := ⟨repr⟩
-
-meta instance has_to_format : has_to_format term := ⟨λ x, repr x⟩
-
-def mk_app (t : term) (ts : list term) : term :=
-list.foldl app t ts
+-- def symb_arity (k : nat) (t : term) : option (bool × nat) :=
+-- symb_arity_core k 0 t
 
 
-@[simp] def fresh_vdx : term → nat
-| (# m)      := m + 1
-| (& _)      := 0
-| (t1 ^* t2) := max t1.fresh_vdx t2.fresh_vdx
 
-def is_fresh_vdx (k : nat) (t : term) : Prop := t.fresh_vdx ≤ k
 
---instance dec_max_idx_lt : ∀ k t, decidable (max_idx_lt k t)
---| := by apply_instance
 
---begin
---  intros k t, induction t;
---  squeeze_simp, repeat {apply_instance},
---  apply @and.decidable _ _ _ _; assumption
---end
-
-@[simp] def val_core (M : model α) (v : nat → α) : term → list α → α
-| (# k)      _  := v k
-| (& k)      as := M.funcs k as
-| (t1 ^* t2) as := t1.val_core (t2.val_core []::as)
-
-def val (M v t) : α := val_core M v t []
-
-def symb_arity_core (k : nat) : nat → term → option (bool × nat)
-| m (# _)    := none
-| m (& n)    := if k = n then some (ff,m) else none
-| m (t ^* s) :=
-  symb_arity_core (m+1) t <|> symb_arity_core 0 s
-
-def symb_arity (k : nat) (t : term) : option (bool × nat) :=
-symb_arity_core k 0 t
-
-def fresh_sdx : term → nat
-| (# _)    := 0
-| (& n)    := n + 1
-| (t ^* s) := max (fresh_sdx t) (fresh_sdx s)
+/- variable index operations  -/
 
 def vdxs : term → list nat
-| (# m)    := [m]
-| (& _)    := []
-| (t ^* s) := vdxs t ∪ vdxs s
+| (⅋ k)   := []
+| (t & s) := vdxs t ∪ vdxs s
+| (t # k) := (vdxs t).insert k
+-- 
+-- def free_vdxs (k : nat) : term → list nat
+-- | (# m)      := if k ≤ m then [m] else []
+-- | (& _)      := []
+-- | (t ^* s) := (free_vdxs t) ∪ (free_vdxs s)
+-- 
+-- def incr_vdx (k : nat) : term → term
+-- | (#m)     := if k ≤ m then #(m + 1) else #m
+-- | (&m)     := (& m)
+-- | (t ^* s) := (incr_vdx t) ^* (incr_vdx s)
+-- 
+-- def fresh_vdx : term → nat
+-- | (# m)      := m + 1
+-- | (& _)      := 0
+-- | (t1 ^* t2) := max t1.fresh_vdx t2.fresh_vdx
+-- 
+-- def is_fresh_vdx (k : nat) (t : term) : Prop := t.fresh_vdx ≤ k
+-- 
+-- 
+/- symbol index operations  -/
 
-def free_vars (k : nat) : term → list nat
-| (# m)      := if k ≤ m then [m] else []
-| (& _)      := []
-| (t ^* s) := (free_vars t) ∪ (free_vars s)
+-- def fresh_sdx : term → nat
+-- | (# _)    := 0
+-- | (& n)    := n + 1
+-- | (t ^* s) := max (fresh_sdx t) (fresh_sdx s)
 
-def subst (m s) : term → term
-| (# k)    := if k = m then s else (# k)
-| (& k)    := (& k)
-| (t ^* u) := (subst t) ^* (subst u)
+end term
 
-def incr_vdx : nat → term → term
-| k (#m)     := if k ≤ m then #(m + 1) else #m
-| k (&m)     := (& m)
-| k (t ^* s) := (incr_vdx k t) ^* (incr_vdx k s)
+
+/- substitution -/
+
+@[reducible] def sub : Type := list (nat × term)
+
+def sub.app (σ : sub) (k : nat) : option term :=
+prod.snd <$> (list.find (eq k ∘ prod.fst)) σ 
+
+namespace term
+
+def subst (σ : sub) : term → term
+| (⅋ k)   := ⅋ k
+| (t & s) := subst t & subst s
+| (t # k) := 
+  match σ.app k with 
+  | none   := subst t # k 
+  | some s := subst t & s 
+  end
+
+lemma subst_eq_of_eq_none {σ : sub} (t : term) {k : nat} :
+σ.app k = none → subst σ (t # k) = subst σ t # k :=
+by { intro h, simp only [h, subst, eq_self_iff_true, and_self] }
+
+lemma subst_eq_of_eq_some {σ : sub} (t s : term) {k : nat} :
+σ.app k = some s → subst σ (t # k) = (subst σ t & s) :=
+by { intro h, simp only [h, subst, eq_self_iff_true, and_self] }
+
+/- evaluation -/
+
+@[simp] def value_core (M : model α) (v : nat → α) : term → list α → α
+| (⅋ k)   as := M.funs k as
+| (t & s) as := t.value_core (s.value_core [] :: as)
+| (t # k) as := t.value_core (v k :: as)
+
+def value (M v t) : α := value_core M v t []
+
+end term
+
+def val.subst (M : model α) (v : nat → α) (σ : sub) (k : nat) : α :=
+match σ.app k with 
+| none   := v k
+| some t := t.value M v  
+end
+
+lemma val.subst_eq_of_eq_none (M : model α) 
+  (v : nat → α) {σ : sub} {k : nat} : 
+σ.app k = none → val.subst M v σ k = v k := 
+by { intro h1, simp only [h1, val.subst] }
+
+lemma val.subst_eq_of_eq_some (M : model α) 
+  (v : nat → α) {σ : sub} {k : nat} {t : term} : 
+σ.app k = some t → val.subst M v σ k = t.value M v := 
+by { intro h1, simp only [h1, val.subst] }
+
+namespace term
+
+lemma value_core_subst (M : model α) (v : nat → α) (σ : sub) :
+  ∀ t : term, ∀ as : list α, 
+  value_core M v (t.subst σ) as = 
+  value_core M (val.subst M v σ) t as  
+| (⅋ k) as   := rfl
+| (t & s) as := 
+  begin
+    have h1 := value_core_subst t, 
+    have h2 := value_core_subst s [], 
+    simp only [value_core, subst, h1, h2]
+  end
+| (t # k) as := 
+  begin
+    cases h1 : σ.app k with s, 
+    simp only [subst_eq_of_eq_none t h1, 
+      val.subst_eq_of_eq_none M v h1,
+      value_core_subst, value_core],
+    simp only [subst_eq_of_eq_some t s h1, 
+      val.subst_eq_of_eq_some M v h1,
+      value_core_subst, value_core, value]
+  end
+
+lemma value_subst (M : model α) (v : nat → α) (σ : sub) (t : term) :
+  value M v (t.subst σ) = value M (val.subst M v σ) t :=  
+by apply value_core_subst
+
+lemma value_comp_subst (M : model α) (v : nat → α) (σ : sub) :
+  value M v ∘ (subst σ) = value M (val.subst M v σ) :=
+function.funext_iff.elim_right (by apply value_subst)
+
+#exit
+
+    simp only [value_core, subst, var.subst, val.subst], 
+  end
+  
 
 #exit
 
